no one reads this anyway

main.lean
@@ -1,18 +1,13 @@
 import tactic.finish
 import tactic.ext
 import biject
+import data.int.parity
 
-universes u1 u2 u3
+universes u1 u2 u3 u4
 
 
 def denombrable (α : Sort u1) : Prop := 
   in_bijection ℕ α
-
-
-def prod_func_left {A : Sort u1} {B : Sort u2}  (f : A → B) (C : Sort u3) : pprod A C → pprod B C :=
-  λ x : pprod A C , pprod.mk (f (x.fst))  x.snd
-
-
 
 theorem tf_l {A : Sort u1} {B : Sort u2} {x3 x4 :pprod A  B} : x3 = x4 →  x3.1 = x4.1 ∧ x3.2 = x4.2 :=
   begin
@@ -42,35 +37,50 @@ theorem tf  {A : Sort u1} {B : Sort u2} (x3 x4 :pprod A  B) : x3 = x4 ↔  x3.1 
   end
 
 
+def prod_func {A : Sort u1} {B : Sort u2} {C : Sort u3} 
+{D : Sort u4} (f : A → B) (g : C → D) : pprod A C → pprod B D :=
+  λ x : pprod A C , pprod.mk (f (x.fst))  (g x.snd)
 
-theorem prod_bij_prod_left {A : Sort u1} {B : Sort u2} (f : A → B) (C : Sort u3) [bijective f]  :
-  bijective (prod_func_left f C) :=
+
+
+
+theorem prod_bij_prod_left {A : Sort u1} {B : Sort u2} {C : Sort u3} 
+{D : Sort u4} (f : A → B) (g : C → D) [bijective f] [bijective g] :
+  bijective (prod_func f g) :=
   begin
     apply and.intro,
       intros x1 x2,
-      rewrite prod_func_left,
+      rewrite prod_func,
       simp,
       intro h,
       apply iff.elim_right (tf x1 x2),
       apply and.intro,
       apply _inst_1.left x1.fst x2.fst
-          ((tf (prod_func_left f C x1) (prod_func_left f C x2)).elim_left h).left,
-        rewrite (tf_l h).elim_right,
+          ((tf (prod_func f g x1) (prod_func f g x2)).elim_left h).left,
+      apply _inst_2.left x1.snd x2.snd
+          ((tf (prod_func f g x1) (prod_func f g x2)).elim_left h).right,
 
     intro y,
     let x1 := (_inst_1.elim_right y.1).some,
-    use pprod.mk x1 y.2,
-    rewrite prod_func_left,
+    let x2 := (_inst_2.elim_right y.2).some,
+    use pprod.mk x1 x2,
+    rewrite prod_func,
     simp,
     apply tf_r,
     simp,
     change x1 with (_inst_1.elim_right y.1).some,
+    change x2 with (_inst_2.elim_right y.2).some,
+    split,
     apply Exists.some_spec (_inst_1.elim_right y.1),
+    apply Exists.some_spec (_inst_2.elim_right y.2)
   end 
+
+
+
 
 theorem Z_denumbrable : denombrable ℤ :=
   begin
-    let f : ℕ → ℤ  := λ n: ℕ , if is_odd
+    let f : ℕ → ℤ  := λ n: ℕ 
 
   end
 
